progs/spec_sha.v
@@ -1,0 +1,323 @@
+Require Import floyd.proofauto.
+Require Import progs.sha.
+Require Import progs.SHA256.
+Require Import progs.sha_lemmas.
+Local Open Scope logic.
+
+Definition __builtin_read32_reversed_spec :=
+ DECLARE ___builtin_read32_reversed
+  WITH p: val, sh: share, contents: Z -> int
+  PRE [ 1%positive OF tptr tuint ] 
+        PROP() LOCAL (`(eq p) (eval_id 1%positive))
+        SEP (`(array_at tuchar sh (cSome contents) 0 4 p))
+  POST [ tuint ] 
+     local (`(eq (Vint (big_endian_integer contents))) retval) &&
+     `(array_at tuchar sh (cSome contents) 0 4 p).
+
+Definition __builtin_write32_reversed_spec :=
+ DECLARE ___builtin_write32_reversed
+  WITH p: val, sh: share, contents: Z -> int
+  PRE [ 1%positive OF tptr tuint, 2%positive OF tuint ] 
+        PROP(writable_share sh)
+        LOCAL (`(eq p) (eval_id 1%positive);
+                     `(eq (Vint(big_endian_integer contents))) (eval_id 2%positive))
+        SEP (`(memory_block sh (Int.repr 4) p))
+  POST [ tvoid ] 
+     `(array_at tuchar sh (cSome contents) 0 4 p).
+
+Definition memcpy_spec :=
+  DECLARE _memcpy
+   WITH sh : share*share, p: val, q: val, n: Z, contents: Z -> int 
+   PRE [ 1%positive OF tptr tvoid, 2%positive OF tptr tvoid, 3%positive OF tuint ]
+       PROP (writable_share (snd sh))
+       LOCAL (`(eq p) (eval_id 1%positive); `(eq q) (eval_id 2%positive);
+                    `(eq n) (`Int.unsigned (`force_int (eval_id 3%positive))))
+       SEP (`(array_at tuchar (fst sh) (cSome contents) 0 n q);
+              `(memory_block (snd sh) (Int.repr n) p))
+    POST [ tptr tvoid ]
+         local (`(eq p) retval) &&
+       (`(array_at tuchar (fst sh) (cSome contents) 0 n q) *
+        `(array_at tuchar (snd sh) (cSome contents) 0 n p)).
+
+Definition memset_spec :=
+  DECLARE _memset
+   WITH sh : share, p: val, n: Z, c: int 
+   PRE [ 1%positive OF tptr tvoid, 2%positive OF tint, 3%positive OF tuint ]
+       PROP (writable_share sh)
+       LOCAL (`(eq p) (eval_id 1%positive); `(eq (Vint c)) (eval_id 2%positive);
+                    `(eq n) (`Int.unsigned (`force_int (eval_id 3%positive))))
+       SEP (`(memory_block sh (Int.repr n) p))
+    POST [ tptr tvoid ]
+         local (`(eq p) retval) &&
+       (`(array_at tuchar sh (fun _ => Some c) 0 n p)).
+
+Goal forall c r,  typed_mapsto Tsh t_struct_SHA256state_st c r = TT.
+ intros.
+ simpl in r.
+ simpl_typed_mapsto.
+ destruct r as [r_h [r_Nl [r_Nh [r_data r_num]]]].
+ simpl.
+Abort.
+
+Definition sha256state_ (a: s256abs) (c: val) : mpred :=
+   EX r:s256state, 
+    !!  s256_relate a r  &&  typed_mapsto Tsh t_struct_SHA256state_st c r.
+
+Definition data_block (contents: list Z) (v: val) :=
+  array_at tuchar Tsh (ZnthV tuchar (map Int.repr contents)) 0 (Zlength contents) v.
+
+Lemma datablock_local_facts:
+ forall f data,
+  data_block f data |-- !! (isptr data).
+Admitted.
+Hint Resolve datablock_local_facts : saturate_local.
+
+Definition sha256_block_data_order_spec :=
+  DECLARE _sha256_block_data_order
+    WITH a: s256abs, b: list int, ctx : val, data: val, sh: share
+   PRE [ _ctx OF tptr t_struct_SHA256state_st, _in OF tptr tvoid ]
+         PROP(length b = LBLOCK) 
+         LOCAL (`(eq ctx) (eval_id _ctx); `(eq data) (eval_id _in))
+         SEP (`(sha256state_ a ctx); `(data_block (intlist_to_Zlist b) data);
+                `(array_at tuint Tsh (ZnthV tuint K) 0 (Zlength K)) (eval_var _K256 (tarray tuint 64)))
+   POST [ tvoid ]
+          (`(sha256state_ (process_block_abs b a) ctx) *
+          `(data_block (intlist_to_Zlist b) data) *
+          `(array_at tuint Tsh (ZnthV tuint K) 0 (Zlength K)) (eval_var _K256 (tarray tuint 64))).
+                
+Definition SHA256_addlength_spec :=
+ DECLARE _SHA256_addlength
+ WITH len : nat, a: s256abs, c: val
+ PRE [ _c OF tptr t_struct_SHA256state_st , _len OF tuint ]
+   PROP ( ) 
+   LOCAL (`(eq (Z.of_nat len)) (`Int.unsigned (`force_int (eval_id _len))); `(eq c) (eval_id _c))
+   SEP(`(sha256state_ a c))
+ POST [ tvoid ]
+   SEP(`(sha256state_ (addlength_rel len a) c)).
+
+Definition SHA256_Init_spec :=
+  DECLARE _SHA256_Init
+   WITH c : val 
+   PRE [ _c OF tptr t_struct_SHA256state_st ]
+         PROP () LOCAL (`(eq c) (eval_id _c))
+         SEP(`(typed_mapsto_ Tsh t_struct_SHA256state_st c))
+  POST [ tvoid ] 
+         SEP(`(sha256state_ init_s256abs c)).
+
+Inductive update_abs: forall (msg: list Z) (a a': s256abs), Prop :=
+| UA_short: forall msg hashed data
+         (H: length (data++msg) < CBLOCK),
+         update_abs msg 
+           (S256abs hashed 0 data)
+           (S256abs hashed 0 (data++msg))
+| UA_long: forall (msg newblock: list Z) (b: list int) hashed data (msg': list Z) a'',
+        newblock = firstn CBLOCK (data++msg) ->
+        intlist_to_Zlist b = newblock ->
+        newblock ++ msg' = data ++ msg ->
+        update_abs msg' (S256abs (hashed++b) 0 nil)   a'' ->
+        update_abs msg (S256abs hashed 0 data) a''.
+
+Definition SHA256_Update_spec :=
+  DECLARE _SHA256_Update
+   WITH a: s256abs, data: list Z, c : val, d: val, sh: share, len : nat
+   PRE [ _c OF tptr t_struct_SHA256state_st, _data_ OF tptr tvoid, _len OF tuint ]
+         PROP ((len <= length data)%nat)
+         LOCAL (`(eq c) (eval_id _c); `(eq d) (eval_id _data_); 
+                                  `(eq (Z.of_nat len)) (`Int.unsigned (`force_int (eval_id _len))))
+         SEP(`(sha256state_ a c); `(data_block data d))
+  POST [ tvoid ] 
+         EX a':_, 
+          PROP (update_abs data a a') LOCAL ()
+          SEP(`(sha256state_ a' c); `(data_block data d)).
+
+Definition s256a_regs (a: s256abs) : list int :=
+ match a with S256abs hashed _ _  => 
+          process_msg init_registers hashed 
+ end.
+
+Definition SHA256_Final_spec :=
+  DECLARE _SHA256_Final
+   WITH a: s256abs, md: val, c : val,  shmd: share, sh: share
+   PRE [ _md OF tptr tuchar, _c OF tptr t_struct_SHA256state_st ]
+         PROP (writable_share shmd) 
+         LOCAL (`(eq md) (eval_id _md); `(eq c) (eval_id _c))
+         SEP(`(sha256state_ a c); `(memory_block shmd (Int.repr 32) md))
+  POST [ tvoid ] 
+         EX a':s256abs,
+         PROP (sha_finish a a') LOCAL ()
+         SEP(`(sha256state_ a' c); `(data_block (intlist_to_Zlist (s256a_regs a')) md)).
+
+Definition SHA256_spec :=
+  DECLARE _SHA256
+   WITH d: val, len: Z, sh: share*share, data: list Z, md: val
+   PRE [ _d OF tptr tuchar, _n OF tuint, _md OF tptr tuchar ]
+         PROP (writable_share (snd sh)) 
+         LOCAL (`(eq d) (eval_id _data_);
+                     `(eq (Z.of_nat (length data))) (`Int.unsigned (`force_int (eval_id _n)));
+                     `(eq md) (eval_id _md))
+         SEP(`(data_block data d);
+               `(memory_block (snd sh) (Int.repr 32) md))
+  POST [ tvoid ] 
+         SEP(`(data_block data d); 
+               `(data_block (SHA_256 data) md)).
+
+Definition Vprog : varspecs := (_K256, tarray tuint 64)::nil.
+
+Definition Gprog : funspecs := 
+  __builtin_read32_reversed_spec::
+  __builtin_write32_reversed_spec::
+  memcpy_spec:: memset_spec::
+  sha256_block_data_order_spec:: SHA256_Init_spec::
+  SHA256_addlength_spec::
+  SHA256_Update_spec:: SHA256_Final_spec::
+  SHA256_spec:: nil.
+
+Fixpoint do_builtins (n: nat) (defs : list (ident * globdef fundef type)) : funspecs :=
+ match n, defs with
+  | S n', (id, Gfun (External (EF_builtin _ sig) argtys resty))::defs' => 
+     (id, mk_funspec (iota_formals 1%positive argtys, resty) unit FF FF) 
+      :: do_builtins n' defs'
+  | _, _ => nil
+ end.
+
+Definition Gtot := do_builtins 3 (prog_defs prog) ++ Gprog.
+
+Lemma sha256state__isptr:
+ forall a c, sha256state_ a c = !!(isptr c) && sha256state_ a c.
+Proof.
+intros. unfold sha256state_. normalize. apply f_equal.
+extensionality r.
+rewrite <- andp_assoc.
+rewrite (andp_comm (!!isptr c)).
+rewrite andp_assoc.
+f_equal.
+simpl_typed_mapsto.
+rewrite field_mapsto_isptr at 1. normalize.
+Qed.
+
+Ltac simpl_stackframe_of := 
+  unfold stackframe_of, fn_vars; simpl map; unfold fold_right; rewrite sepcon_emp;
+  repeat rewrite var_block_typed_mapsto_. 
+
+Fixpoint loops (s: statement) : list statement :=
+ match s with 
+  | Ssequence a b => loops a ++ loops b
+  | Sloop _ _ => [s]
+  | Sifthenelse _ a b => loops a ++ loops b
+  | _ => nil
+  end.
+
+Definition rearrange_regs :=
+(Ssequence
+     (Sset _T1
+        (Ebinop Oadd
+           (Ebinop Oadd
+              (Ebinop Oadd
+                 (Ebinop Oadd (Etempvar _l tuint) (Etempvar _h tuint) tuint)
+                 (Ebinop Oxor
+                    (Ebinop Oxor
+                       (Ebinop Oor
+                          (Ebinop Oshl (Etempvar _e tuint)
+                             (Econst_int (Int.repr 26) tint) tuint)
+                          (Ebinop Oshr
+                             (Ebinop Oand (Etempvar _e tuint)
+                                (Econst_int (Int.repr (-1)) tuint) tuint)
+                             (Ebinop Osub (Econst_int (Int.repr 32) tint)
+                                (Econst_int (Int.repr 26) tint) tint) tuint)
+                          tuint)
+                       (Ebinop Oor
+                          (Ebinop Oshl (Etempvar _e tuint)
+                             (Econst_int (Int.repr 21) tint) tuint)
+                          (Ebinop Oshr
+                             (Ebinop Oand (Etempvar _e tuint)
+                                (Econst_int (Int.repr (-1)) tuint) tuint)
+                             (Ebinop Osub (Econst_int (Int.repr 32) tint)
+                                (Econst_int (Int.repr 21) tint) tint) tuint)
+                          tuint) tuint)
+                    (Ebinop Oor
+                       (Ebinop Oshl (Etempvar _e tuint)
+                          (Econst_int (Int.repr 7) tint) tuint)
+                       (Ebinop Oshr
+                          (Ebinop Oand (Etempvar _e tuint)
+                             (Econst_int (Int.repr (-1)) tuint) tuint)
+                          (Ebinop Osub (Econst_int (Int.repr 32) tint)
+                             (Econst_int (Int.repr 7) tint) tint) tuint)
+                       tuint) tuint) tuint)
+              (Ebinop Oxor
+                 (Ebinop Oand (Etempvar _e tuint) (Etempvar _f tuint) tuint)
+                 (Ebinop Oand (Eunop Onotint (Etempvar _e tuint) tuint)
+                    (Etempvar _g tuint) tuint) tuint) tuint)
+           (Etempvar _Ki tuint) tuint))
+     (Ssequence
+        (Sset _T2
+           (Ebinop Oadd
+              (Ebinop Oxor
+                 (Ebinop Oxor
+                    (Ebinop Oor
+                       (Ebinop Oshl (Etempvar _a tuint)
+                          (Econst_int (Int.repr 30) tint) tuint)
+                       (Ebinop Oshr
+                          (Ebinop Oand (Etempvar _a tuint)
+                             (Econst_int (Int.repr (-1)) tuint) tuint)
+                          (Ebinop Osub (Econst_int (Int.repr 32) tint)
+                             (Econst_int (Int.repr 30) tint) tint) tuint)
+                       tuint)
+                    (Ebinop Oor
+                       (Ebinop Oshl (Etempvar _a tuint)
+                          (Econst_int (Int.repr 19) tint) tuint)
+                       (Ebinop Oshr
+                          (Ebinop Oand (Etempvar _a tuint)
+                             (Econst_int (Int.repr (-1)) tuint) tuint)
+                          (Ebinop Osub (Econst_int (Int.repr 32) tint)
+                             (Econst_int (Int.repr 19) tint) tint) tuint)
+                       tuint) tuint)
+                 (Ebinop Oor
+                    (Ebinop Oshl (Etempvar _a tuint)
+                       (Econst_int (Int.repr 10) tint) tuint)
+                    (Ebinop Oshr
+                       (Ebinop Oand (Etempvar _a tuint)
+                          (Econst_int (Int.repr (-1)) tuint) tuint)
+                       (Ebinop Osub (Econst_int (Int.repr 32) tint)
+                          (Econst_int (Int.repr 10) tint) tint) tuint) tuint)
+                 tuint)
+              (Ebinop Oxor
+                 (Ebinop Oxor
+                    (Ebinop Oand (Etempvar _a tuint) (Etempvar _b tuint)
+                       tuint)
+                    (Ebinop Oand (Etempvar _a tuint) (Etempvar _c tuint)
+                       tuint) tuint)
+                 (Ebinop Oand (Etempvar _b tuint) (Etempvar _c tuint) tuint)
+                 tuint) tuint))
+        (Ssequence (Sset _h (Etempvar _g tuint))
+           (Ssequence (Sset _g (Etempvar _f tuint))
+              (Ssequence (Sset _f (Etempvar _e tuint))
+                 (Ssequence
+                    (Sset _e
+                       (Ebinop Oadd (Etempvar _d tuint) (Etempvar _T1 tuint)
+                          tuint))
+                    (Ssequence (Sset _d (Etempvar _c tuint))
+                       (Ssequence (Sset _c (Etempvar _b tuint))
+                          (Ssequence (Sset _b (Etempvar _a tuint))
+                             (Sset _a
+                                (Ebinop Oadd (Etempvar _T1 tuint)
+                                   (Etempvar _T2 tuint) tuint))))))))))).
+
+
+Definition Delta_loop1 : tycontext :=
+ initialized _i
+          (initialized _h
+           (initialized _g
+              (initialized _f
+                 (initialized _e
+                    (initialized _d
+                       (initialized _c
+                          (initialized _b
+                             (initialized _a
+                                (initialized _data
+     (func_tycontext f_sha256_block_data_order Vprog Gtot)))))))))).
+
+
+
+
+
+
