progs/verif_sha_bdo.v
@@ -1,0 +1,665 @@
+Require Import floyd.proofauto.
+Require Import progs.sha.
+Require Import progs.SHA256.
+Require Import progs.sha_lemmas.
+Require Import progs.spec_sha.
+Require Import progs.verif_sha_bdo2.
+Require Import progs.verif_sha_bdo3.
+Local Open Scope logic.
+
+Definition block_data_order_loop1 := 
+   nth 0 (loops (fn_body f_sha256_block_data_order)) Sskip.
+
+Definition block_data_order_loop2 := 
+   nth 1 (loops (fn_body f_sha256_block_data_order)) Sskip.
+
+Lemma read32_reversed_in_bytearray:
+ forall {Espec: OracleKind} Delta (ofs: int) (lo hi: Z) base e sh contents i P Q
+ (VS:  (var_types Delta) ! ___builtin_read32_reversed = None) 
+ (GS: (glob_types Delta) ! ___builtin_read32_reversed =
+    Some (Global_func (snd __builtin_read32_reversed_spec)))
+ (TE: typeof e = tptr tuint)
+ (CLOQ: Forall (closed_wrt_vars (eq i)) Q)
+ (Hcontents: forall i, (lo <= i < hi)%Z -> isSome (contents i)),
+ PROPx P (LOCALx (tc_environ Delta :: Q) (SEP (TT))) |-- PROP ((lo <= Int.unsigned ofs <= hi-4 )%Z)
+         LOCAL (tc_expr Delta e; `(eq (offset_val ofs base)) (eval_expr e))
+         SEP  (TT) ->
+ semax Delta  (PROPx P (LOCALx Q (SEP (`(array_at tuchar sh contents lo hi base)))))
+        (Scall (Some i)
+           (Evar ___builtin_read32_reversed
+              (Tfunction (Tcons (tptr tuint) Tnil) tuint))
+           [e])
+        (normal_ret_assert
+         (PROP () 
+         (LOCALx (`(eq (Vint (big_endian_integer (fun z => force_option Int.zero (contents (z+Int.unsigned ofs)%Z))))) (eval_id i)
+                        :: Q)                 
+         SEP (`(array_at tuchar sh contents lo hi base))))).
+Proof.
+intros.
+apply semax_pre with
+ (PROP  ((lo <= Int.unsigned ofs <= hi - 4)%Z)
+        (LOCALx (tc_expr Delta e :: `(eq (offset_val ofs base)) (eval_expr e) :: Q)
+         (SEP(`(array_at tuchar sh contents lo hi base))))).
+rewrite <- (andp_dup (PROPx P _)).
+eapply derives_trans; [ apply andp_derives | ].
+eapply derives_trans; [ | apply H].
+apply andp_derives; auto.
+apply andp_derives; auto.
+go_lowerx.
+apply sepcon_derives; auto.
+apply TT_right.
+instantiate (1:= PROPx nil (LOCALx Q (SEP  (`(array_at tuchar sh contents lo hi base))))).
+go_lowerx. entailer.
+go_lowerx; entailer.
+normalize.
+clear H.
+normalize.
+rewrite (split_array_at (Int.unsigned ofs)) by omega.
+rewrite (split_array_at (Int.unsigned ofs + 4)%Z) with (hi:=hi) by omega.
+normalize.
+match goal with |- semax _ (PROPx _ (LOCALx _ ?A)) _ _ =>
+ replace A  with (SEPx( [
+         `(array_at tuchar sh contents (Int.unsigned ofs)
+             (Int.unsigned ofs + 4) base)] ++
+               [`(array_at tuchar sh contents lo (Int.unsigned ofs) base),
+         `(array_at tuchar sh contents (Int.unsigned ofs + 4) hi base)]))
+ by (simpl app; apply pred_ext; go_lowerx; cancel)
+end.
+eapply semax_frame1; try reflexivity;
+ [ |  apply derives_refl | auto 50 with closed].
+eapply semax_pre_post.
+Focus 3.
+evar (tl: typelist).
+replace (Tcons (tptr tuint) Tnil) with tl.
+unfold tl.
+eapply semax_call_id1'; try eassumption.
+2: reflexivity.
+apply GS.
+2: reflexivity.
+Unfocus.
+instantiate (3:=nil).
+apply andp_left2.
+instantiate (2:=(offset_val ofs base, sh, fun z => force_option Int.zero (contents (z + Int.unsigned ofs)%Z))).
+cbv beta iota.
+instantiate (1:=nil).
+unfold split; simpl @snd.
+go_lowerx.
+entailer.
+apply andp_right; [apply prop_right; repeat split; auto | ].
+hnf. simpl.
+rewrite TE.
+repeat rewrite denote_tc_assert_andp; repeat split; auto.
+rewrite <- H3.
+rewrite TE.
+destruct base; inv Pbase; reflexivity.
+pattern ofs at 4;
+ replace ofs with (Int.repr (sizeof tuchar * Int.unsigned ofs))%Z
+ by (simpl sizeof; rewrite Z.mul_1_l; apply Int.repr_unsigned).
+rewrite <- offset_val_array_at.
+apply derives_refl'.
+apply equal_f. rewrite Z.add_0_r. apply array_at_ext.
+intros. unfold cSome. rewrite Z.sub_add.
+clear - H5 H0 Hcontents.
+specialize (Hcontents i0);
+ destruct (contents i0); [ | elimtype False; apply Hcontents; omega]. reflexivity.
+2: auto with closed.
+intros; apply andp_left2.
+apply normal_ret_assert_derives'.
+go_lowerx.
+entailer.
+apply derives_refl'.
+pattern ofs at 2;
+ replace ofs with (Int.repr (sizeof tuchar * Int.unsigned ofs))%Z
+ by (simpl sizeof; rewrite Z.mul_1_l; apply Int.repr_unsigned).
+rewrite <- offset_val_array_at.
+apply equal_f. rewrite Z.add_0_r. 
+apply array_at_ext; intros.
+unfold cSome. rewrite Z.sub_add.
+clear - H3 H0 Hcontents.
+specialize (Hcontents i0); destruct (contents i0);
+  [reflexivity | contradiction Hcontents; omega].
+Qed.
+
+Definition f_upto {A} (f: Z -> option A) (bound: Z) (i: Z) : option A :=
+ if zlt i bound then f i else None.
+
+Lemma array_at_f_upto_lo:
+  forall t sh contents lo hi, 
+  array_at t sh (f_upto contents lo) lo hi = array_at_ t sh lo hi.
+Proof.
+intros; apply array_at_ext; intros.
+unfold f_upto; if_tac; auto. omega.
+Qed.
+
+Lemma sha256_block_data_order_loop1_proof:
+  forall (Espec : OracleKind)
+     (b: list int) (data: val) (regs: list int)
+     (Hdata: isptr data),
+     length b = LBLOCK ->
+     semax Delta_loop1
+  (PROP ()
+   LOCAL (`(eq (Vint (Int.repr 0))) (eval_id _i);
+               `(eq data) (eval_id _data);
+               `(eq (map Vint regs)) 
+                  (`cons (eval_id _a) (`cons (eval_id _b) (`cons (eval_id _c) (`cons (eval_id _d)
+                   (`cons (eval_id _e) (`cons (eval_id _f) (`cons (eval_id _g) (`cons (eval_id _h) `nil)))))
+))))
+   SEP ( `(array_at tuint Tsh (ZnthV tuint K) 0 (Zlength K)) (eval_var _K256 (tarray tuint 64));
+           `(array_at_ tuint Tsh 0 16) (eval_var _X (tarray tuint 16));
+           `(data_block (intlist_to_Zlist (map swap b)) data)))
+  block_data_order_loop1
+  (normal_ret_assert
+    (PROP () 
+     LOCAL(`(eq (map Vint (rnd_64 regs K b))) 
+                   (`cons (eval_id _a) (`cons (eval_id _b) (`cons (eval_id _c) (`cons (eval_id _d)
+                     (`cons (eval_id _e) (`cons (eval_id _f) (`cons (eval_id _g) (`cons (eval_id _h) `nil)))))
+))))
+     SEP ( `(array_at tuint Tsh (ZnthV tuint K) 0 (Zlength K)) (eval_var _K256 (tarray tuint 64));
+           `(array_at tuint Tsh (ZnthV tuint b) 0 16) (eval_var _X (tarray tuint 16));
+           `(data_block (intlist_to_Zlist (map swap b)) data))) ).
+Proof.
+unfold block_data_order_loop1, Delta_loop1.
+intros.
+simpl nth; fold rearrange_regs.
+abbreviate_semax.
+name a_ _a.
+name b_ _b.
+name c_ _c.
+name d_ _d.
+name e_ _e.
+name f_ _f.
+name g_ _g.
+name h_ _h.
+name l_ _l.
+name l'_ _l'.
+name Ki _Ki.
+name in_ _in.
+name ctx_ _ctx.
+name i_ _i.
+name data_ _data.
+assert (LBE := LBLOCK_zeq).
+
+Definition loop1_inv (rg0: list int) (b: list int) (data: val) (delta: Z) (i: nat) :=
+    PROP ( i <= 16 )
+    LOCAL  (`(eq (Vint (Int.repr (Z.of_nat i - delta)))) (eval_id _i);
+               `(eq (offset_val (Int.repr ((Z.of_nat i)*4)) data)) (eval_id _data);
+     `(eq (map Vint (rnd_64 rg0 K (firstn i b))))
+      (`cons (eval_id _a)
+         (`cons (eval_id _b)
+            (`cons (eval_id _c)
+               (`cons (eval_id _d)
+                  (`cons (eval_id _e)
+                     (`cons (eval_id _f)
+                        (`cons (eval_id _g) (`cons (eval_id _h) `[])))))))))
+     SEP (`(array_at tuint Tsh (ZnthV tuint K) 0 (Zlength K))
+      (eval_var _K256 (tarray tuint 64));
+    `(array_at tuint Tsh (f_upto (ZnthV tuint b) (Z.of_nat i) ) 0 (Z.of_nat LBLOCK)) (eval_var _X (tarray tuint 16));
+   `(data_block (intlist_to_Zlist (map swap b)) data)).
+
+apply semax_pre with (EX i:nat, loop1_inv regs b data 0 i).
+(* 345,184   326,392*)
+abstract (unfold loop1_inv;
+          apply exp_right with 0;
+          rewrite array_at_f_upto_lo;
+          entailer!; omega).
+(* 419,452   431,980 *)
+apply semax_post' with (loop1_inv regs b data 0 LBLOCK).
+(* 419,452  431,980 *)
+abstract (unfold loop1_inv;
+               entailer! ;
+           rewrite <- H2; repeat f_equal; 
+           symmetry; apply firstn_same; omega).
+(* 445,728  479,964 *)
+clear POSTCONDITION.
+apply (semax_loop _ _ (EX i:nat, loop1_inv regs b data 1 i)).
+2: abstract (
+apply extract_exists_pre; intro i;
+forward;  (*  i += 1; *)
+apply exp_right with i;
+(* 452,280  481,476 *)
+ unfold loop1_inv;  entailer! ; f_equal; omega).
+(* 561,900  574,392 *)
+
+apply extract_exists_pre; intro i.
+unfold loop1_inv.
+forward_if (
+PROP  (i < 16)
+   LOCAL  (`(eq (Vint (Int.repr (Z.of_nat (0 + i))))) (eval_id _i);
+               `(eq (offset_val (Int.repr ((Z.of_nat i)*4)) data)) (eval_id _data);
+   `(eq (map Vint (rnd_64 regs K (firstn i b))))
+     (`cons (eval_id _a)
+        (`cons (eval_id _b)
+           (`cons (eval_id _c)
+              (`cons (eval_id _d)
+                 (`cons (eval_id _e)
+                    (`cons (eval_id _f)
+                       (`cons (eval_id _g) (`cons (eval_id _h) `[])))))))))
+   SEP 
+   (`(array_at tuint Tsh (ZnthV tuint K) 0 (Zlength K))
+      (eval_var _K256 (tarray tuint 64));
+   `(array_at tuint Tsh (f_upto (ZnthV tuint b) (Z.of_nat i)) 0 (Z.of_nat LBLOCK)) (eval_var _X (tarray tuint 16));
+   `(data_block (intlist_to_Zlist (map swap b)) data))).
+(* 587,640  592,608 *)
+abstract entailer.
+(* 613,416  655,716 *)
+abstract (forward; (* skip; *)
+(* 619,968  655,716 *)
+   entailer; apply prop_right; clear - H2; split; [omega | f_equal; omega]).
+(* 726,056  709,784 *)
+abstract (forward;  (* break; *)
+(* 738,188  709,784 *)
+  entailer; 
+ assert (i=16) by omega; subst i; 
+ apply andp_right; [ apply prop_right | cancel];
+ replace 16 with LBLOCK in H3 by omega;
+ repeat split; auto).
+(* 854,860 750,176 *)
+unfold MORE_COMMANDS, POSTCONDITION, abbreviate;
+ clear MORE_COMMANDS POSTCONDITION.
+make_sequential.
+unfold loop1_ret_assert.
+apply extract_exists_post with (S i).
+rewrite inj_S.
+simpl plus.
+normalize.
+
+(* 945,760 834,556 *)
+
+do 2 apply -> seq_assoc.
+eapply semax_frame_seq
+ with (P1 := [])
+         (Q1 :=  [ 
+`(eq (Vint (Int.repr (Z.of_nat i)))) (eval_id _i),
+`(eq (offset_val (Int.repr (Z.of_nat i * 4)) data)) (eval_id _data),
+`(eq (map Vint (rnd_64 regs K (firstn i b))))
+  (`cons (eval_id _a)
+     (`cons (eval_id _b)
+        (`cons (eval_id _c)
+           (`cons (eval_id _d)
+              (`cons (eval_id _e)
+                 (`cons (eval_id _f)
+                    (`cons (eval_id _g) (`cons (eval_id _h) `[]))))))))])
+         (Frame := [`(array_at tuint Tsh (ZnthV tuint K) 0 (Zlength K))
+      (eval_var _K256 (tarray tuint 64)),
+   `(array_at tuint Tsh (f_upto (ZnthV tuint b) (Z.of_nat i)) 0 (Z.of_nat LBLOCK)) (eval_var _X (tarray tuint 16))]); 
+   [apply (read32_reversed_in_bytearray _ (Int.repr (Z.of_nat i * 4)) 0 (Zlength (intlist_to_Zlist (map swap b))) data _ Tsh 
+                     (ZnthV tuchar (map Int.repr (intlist_to_Zlist (map swap b)))));
+    [ reflexivity | reflexivity | reflexivity | auto 50 with closed | 
+      intros; apply ZnthV_isSome; rewrite Zlength_correct, map_length;
+          rewrite Zlength_correct in H1; apply H1
+      | ]
+   | | | ].
+(* 945,760 834,556 *)
+abstract solve [entailer!; repeat split; auto; try omega; 
+ rewrite Zlength_correct; rewrite length_intlist_to_Zlist; 
+            rewrite map_length; rewrite H;
+ replace (Z.of_nat (4 * LBLOCK) - 4)%Z
+  with ((Z.of_nat LBLOCK - 1) * 4)%Z; 
+    [apply Zmult_le_compat_r; omega | ];
+ rewrite Zmult_comm;
+ rewrite Z.mul_sub_distr_l;
+ reflexivity].
+(* 990,216 849,172 *)
+abstract solve [entailer!].
+(* 1,078,128 849,172 *)
+auto 50 with closed.
+simpl.
+change (array_at tuchar Tsh (ZnthV tuchar (map Int.repr (intlist_to_Zlist (map swap b)))) 0
+        (Zlength (intlist_to_Zlist (map swap b))) data)
+  with (data_block  (intlist_to_Zlist (map swap b)) data).
+
+forward. (* l := l'; *)
+forward. (* data := data + 4; *)
+(* 1,194,800 849,172 *)
+abstract solve [entailer!].
+(* 1,254,920 849,172 *)
+normalize.
+(* 1,291,784 894,136 *)
+simpl typeof.
+forward. (* X[i]=l; *)
+clear POSTCONDITION MORE_COMMANDS.
+instantiate (2:= Z.of_nat i).
+instantiate (1:= big_endian_integer
+          (fun z : Z =>
+           force_option Int.zero
+             (ZnthV tuchar (map Int.repr (intlist_to_Zlist (map swap b)))
+                (z + Z.of_nat i * 4)))).
+abstract (entailer; apply prop_right; repeat split; try omega; eapply eval_var_isptr; eauto).
+
+rewrite <- (array_at_ext tuint Tsh 
+    (f_upto (ZnthV tuint b) (Z.of_nat (S i)))
+     (upd (f_upto (ZnthV tuint b) (Z.of_nat i)) (Z.of_nat i)
+             (Some (big_endian_integer
+          (fun z : Z =>
+           force_option Int.zero
+             (ZnthV tuchar (map Int.repr (intlist_to_Zlist (map swap b)))
+                (z + Z.of_nat i * 4)))))))
+ by abstract (
+ intros; unfold upd; if_tac; unfold f_upto;
+ [rewrite if_true by (rewrite inj_S; omega);
+  unfold ZnthV; rewrite <- H2; rewrite Nat2Z.id;
+  rewrite <- nth_big_endian_int; [ reflexivity | omega ]
+ | unfold f_upto; rewrite inj_S; if_tac; if_tac; auto; omega]).
+(* 1,506,948 1,110,852 *)
+(* 1,506,948 1,134,576 *)
+assert (isSome (ZnthV tuint K (Z.of_nat i))) 
+ by abstract (clear - H0; apply ZnthV_isSome;
+        split; try omega; apply Z.lt_trans with 16%Z; [omega | compute; auto]).
+clear H1.
+forward.  (* Ki=K256[i]; *)
+(* 1,689,280 1,212,872 *)
+abstract (
+assert (Zlength K = 64%Z) by reflexivity;
+entailer!; try apply_ZnthV_isSome; try omega;
+ eapply eval_var_isptr; eauto).
+(* 1,811,028 1,406,332 *)
+unfold POSTCONDITION, abbreviate; clear POSTCONDITION.
+
+match goal with 
+  |- semax _ (PROPx _ (LOCALx _ (SEPx ?R))) _ 
+       (normal_ret_assert (PROPx ?P (LOCALx ?Q _)))
+ => apply semax_post' with (PROPx P (LOCALx Q (SEPx R)));
+  [ | change R with (nil++R); apply semax_frame_PQR with (R2:=R)]
+end.
+abstract (
+apply andp_derives; auto;
+apply andp_derives; auto;
+unfold Z.succ; rewrite inj_S;
+go_lower0; cancel).
+auto 50 with closed.
+(* 1,811,028 1,429,048 *)
+change (match b with
+                | [] => []
+                | a :: l => a :: firstn i l
+                end) with (firstn (S i) b).
+eapply semax_pre; [ | apply rearrange_regs_proof; auto ].
+abstract (entailer!;
+ [destruct data; inv Hdata; simpl; f_equal;
+  rewrite Int.add_assoc;
+  f_equal; unfold Z.succ; rewrite Z.mul_add_distr_r;
+  rewrite <- add_repr;
+  f_equal
+ | unfold ZnthV; simpl; rewrite Nat2Z.id;
+   clear - H0;
+   destruct (assert_lemmas.nth_error_in_bounds K i) as [j ?];
+    [compute; omega | rewrite H; reflexivity]
+ ]).
+(* 2,xxx,xxx 1,579,524 *)
+Qed.
+
+Lemma local_and_retval: (* do we need this? *)
+ forall (i: ident) (P: val -> Prop) (R: mpred),
+    `(local (`P retval) && `R) (get_result1 i) = local (`P (eval_id i)) && `R.
+Proof.
+intros.
+extensionality rho.
+super_unfold_lift.
+unfold get_result1. simpl.
+unfold local, lift1.
+f_equal; auto.
+Qed.
+Hint Rewrite local_and_retval: norm.
+
+Lemma sha256_block_data_order_loop2_proof:
+  forall (Espec : OracleKind)
+     (b: list int) (data: val) (regs: list int),
+     length b = LBLOCK ->
+     semax  Delta_loop1
+ (PROP ()
+   LOCAL (`(eq (map Vint (rnd_64 regs K b))) 
+                   (`cons (eval_id _a) (`cons (eval_id _b) (`cons (eval_id _c) (`cons (eval_id _d)
+                     (`cons (eval_id _e) (`cons (eval_id _f) (`cons (eval_id _g) (`cons (eval_id _h) `nil)))))
+))))
+   SEP ( `(array_at tuint Tsh (ZnthV tuint K) 0 (Zlength K))
+                   (eval_expr (Evar _K256 (tarray tuint 64)));
+           `(array_at tuint Tsh (ZnthV tuint b) 0 16) (eval_var _X (tarray tuint 16))))
+  block_data_order_loop2
+  (normal_ret_assert
+    (PROP () 
+     LOCAL(`(eq (map Vint (rnd_64 regs K (rev (generate_word (rev b) 48)))))
+                   (`cons (eval_id _a) (`cons (eval_id _b) (`cons (eval_id _c) (`cons (eval_id _d)
+                     (`cons (eval_id _e) (`cons (eval_id _f) (`cons (eval_id _g) (`cons (eval_id _h) `nil)))))
+))))
+     SEP ( `(array_at tuint Tsh (ZnthV tuint K) 0 (Zlength K))
+                   (eval_expr (Evar _K256 (tarray tuint 64)));
+           `(array_at_ tuint Tsh 0 16) (eval_var _X (tarray tuint 16))))).
+Admitted.
+
+Lemma semax_seq_congr:  (* not provable *)
+ forall (Espec: OracleKind) s1 s1' s2 s2',
+  (forall Delta P R, semax Delta P s1 R <-> semax Delta P s1' R) ->
+  (forall Delta P R, semax Delta P s2 R <-> semax Delta P s2' R) ->
+ (forall Delta P R, 
+    semax Delta P (Ssequence s1 s2) R <->
+    semax Delta P (Ssequence s1' s2') R).
+Abort.
+
+Definition load8 id ofs :=
+ (Sset id
+      (Ederef
+        (Ebinop Oadd
+          (Efield
+            (Ederef (Etempvar _ctx (tptr t_struct_SHA256state_st))
+              t_struct_SHA256state_st) _h (tarray tuint 8))
+          (Econst_int (Int.repr ofs) tint) (tptr tuint)) tuint)).
+
+Lemma sha256_block_load8:
+  forall (Espec : OracleKind) 
+     (data: val) (r_h: list int) (ctx: val)
+   (H5 : length r_h = 8),
+     semax  
+      (initialized _data
+         (func_tycontext f_sha256_block_data_order Vprog Gtot))
+  (PROP  ()
+   LOCAL  (`eq (eval_id _data) (eval_expr (Etempvar _in (tptr tvoid)));
+   `(eq ctx) (eval_id _ctx); `(eq data) (eval_id _in))
+   SEP  (`(array_at tuint Tsh (ZnthV tuint r_h) 0 (Zlength r_h) ctx)))
+   (Ssequence (load8 _a 0)
+     (Ssequence (load8 _b 1)
+     (Ssequence (load8 _c 2)
+     (Ssequence (load8 _d 3)
+     (Ssequence (load8 _e 4)
+     (Ssequence (load8 _f 5)
+     (Ssequence (load8 _g 6)
+     (Ssequence (load8 _h 7)
+         Sskip))))))))
+  (normal_ret_assert 
+  (PROP  ()
+   LOCAL  (`(eq (map Vint r_h))
+                    (`cons (eval_id _a) (`cons (eval_id _b) (`cons (eval_id _c) (`cons (eval_id _d)
+                     (`cons (eval_id _e) (`cons (eval_id _f) (`cons (eval_id _g) (`cons (eval_id _h) `nil)))))
+)));
+   `eq (eval_id _data) (eval_expr (Etempvar _in (tptr tvoid)));
+   `(eq ctx) (eval_id _ctx); `(eq data) (eval_id _in))
+   SEP  (`(array_at tuint Tsh (ZnthV tuint r_h) 0 (Zlength r_h) ctx)))).
+Proof.
+intros.
+simplify_Delta.
+unfold load8.
+abbreviate_semax.
+normalize.
+simpl.
+normalize.
+name a_ _a.
+name b_ _b.
+name c_ _c.
+name d_ _d.
+name e_ _e.
+name f_ _f.
+name g_ _g.
+name h_ _h.
+name l_ _l.
+name Ki _Ki.
+name in_ _in.
+name ctx_ _ctx.
+name i_ _i.
+name data_ _data.
+abbreviate_semax.
+assert (H5': Zlength r_h = 8%Z).
+rewrite Zlength_correct; rewrite H5; reflexivity.
+do 8 (forward; [ (entailer!; try apply_ZnthV_isSome; omega) | ]).
+forward.  (* skip; *)
+entailer.
+do 9 (destruct r_h as [ | ?h r_h ] ; [inv H5 | ]).
+reflexivity.
+inv H5.
+Qed.
+
+Definition get_h (n: Z) :=
+    Sset _t
+        (Ederef
+           (Ebinop Oadd
+              (Efield
+                 (Ederef (Etempvar _ctx (tptr t_struct_SHA256state_st))
+                    t_struct_SHA256state_st) _h (tarray tuint 8))
+              (Econst_int (Int.repr n) tint) (tptr tuint)) tuint).
+
+Definition add_h (n: Z) (i: ident) :=
+   Sassign
+       (Ederef
+          (Ebinop Oadd
+             (Efield
+                (Ederef (Etempvar _ctx (tptr t_struct_SHA256state_st))
+                   t_struct_SHA256state_st) _h (tarray tuint 8))
+             (Econst_int (Int.repr n) tint) (tptr tuint)) tuint)
+       (Ebinop Oadd (Etempvar _t tuint) (Etempvar i tuint) tuint).
+
+Definition add_them_back :=
+ [get_h 0, add_h 0 _a,
+  get_h 1, add_h 1 _b,
+  get_h 2, add_h 2 _c,
+  get_h 3, add_h 3 _d,
+  get_h 4, add_h 4 _e,
+  get_h 5, add_h 5 _f,
+  get_h 6, add_h 6 _g,
+  get_h 7, add_h 7 _h].
+
+
+Lemma add_them_back_proof:
+  forall (Espec : OracleKind)
+     (b: list int) (r_h: list int)(ctx: val)(hashed: list int),
+     length b = LBLOCK ->
+     semax  Delta_loop1
+   (PROP  ()
+   LOCAL 
+   (`(eq (map Vint (rnd_64 r_h K (rev (generate_word (rev b) 48)))))
+      (`cons (eval_id _a)
+         (`cons (eval_id _b)
+            (`cons (eval_id _c)
+               (`cons (eval_id _d)
+                  (`cons (eval_id _e)
+                     (`cons (eval_id _f)
+                        (`cons (eval_id _g) (`cons (eval_id _h) `[])))))))))
+   SEP 
+   (`(array_at tuint Tsh (ZnthV tuint (process_msg init_registers hashed)) 0
+       (Zlength (process_msg init_registers hashed)) ctx)))
+   (sequence add_them_back Sskip)
+  (normal_ret_assert
+   (PROP() LOCAL() 
+    SEP (`(array_at tuint Tsh (ZnthV tuint 
+                   (map2 Int.add (process_msg init_registers hashed)
+                                         (rnd_64 r_h K (rev (generate_word (rev b) 48)))))
+            0 (Zlength (process_msg init_registers hashed)) ctx)))).
+Admitted.
+
+Hint Extern 2 (array_at _ _ _ _ _ _ |-- array_at_ _ _ _ _ _) =>
+  (apply array_at__array_at; clear; simpl; congruence) : cancel.
+(* move the Hint to malloc_lemmas.v, 
+  and change the name of array_at__array_at to array_at_array_at_
+*)
+
+
+Lemma body_sha256_block_data_order: semax_body Vprog Gtot f_sha256_block_data_order sha256_block_data_order_spec.
+Proof.
+start_function.
+name a_ _a.
+name b_ _b.
+name c_ _c.
+name d_ _d.
+name e_ _e.
+name f_ _f.
+name g_ _g.
+name h_ _h.
+name l_ _l.
+name Ki _Ki.
+name in_ _in.
+name ctx_ _ctx.
+name i_ _i.
+name data_ _data.
+unfold sha256state_.
+simpl_stackframe_of. 
+normalize. intros [r_h [r_Nl [r_Nh [r_data r_num]]]].
+repeat simpl_typed_mapsto.
+unfold fst,snd.
+normalize.
+unfold s256_relate in H1. destruct a.
+simpl in H1.
+unfold s256_Nh, s256_Nl, s256_data, s256_num, fst, snd in H1.
+destruct H1 as [? [? [? [H4 [H4b H4c]]]]].
+destruct H4b as [n H4b].
+change (length hashed = 16 * n)%nat in H4b.
+assert (length r_h = 8%nat) by (subst r_h; apply length_process_msg).
+forward. (* data = in; *)
+abbreviate_semax.
+match goal with |- semax _ (PROPx nil ?QR) _ _ =>
+ apply semax_pre0 with (PROPx [isptr data] QR)
+end.
+apply andp_right; [ | apply andp_left2; auto].
+entailer.
+normalize.
+match goal with |- semax _ _ ?c _ =>
+ eapply seq_assocN with (cs := sequenceN 8 c)
+end.
+eapply semax_frame1.
+eapply sha256_block_load8 with (ctx:=ctx); eassumption.
+simplify_Delta; reflexivity.
+entailer!.
+auto 50 with closed.
+abbreviate_semax.
+simpl.
+do 2 match goal with |- appcontext [lift1 ?A] => 
+  change (lift1 A) with (`A)
+end.
+forward.  (* i = 0; *)
+
+eapply semax_frame_seq.
+replace Delta with Delta_loop1
+ by (simplify_Delta; reflexivity).
+simple apply (sha256_block_data_order_loop1_proof
+  _ b data r_h); auto.
+entailer!.
+auto 50 with closed.
+simpl; abbreviate_semax.
+
+eapply semax_frame_seq.
+apply sha256_block_data_order_loop2_proof
+              with (regs:=r_h)(b:=b); eassumption.
+entailer!.
+auto 50 with closed.
+unfold app; abbreviate_semax.
+eapply seq_assocN with (cs := add_them_back).
+
+eapply semax_frame1.
+apply (add_them_back_proof _ b r_h ctx hashed); try eassumption.
+simplify_Delta; reflexivity.
+entailer. cancel.
+auto 50 with closed.
+simpl; abbreviate_semax.
+
+simpl.
+do 2 match goal with |- appcontext [lift1 ?A] => 
+  change (lift1 A) with (`A)
+end.
+unfold POSTCONDITION, abbreviate; clear POSTCONDITION.
+eapply sha256_block_data_order_return; eauto.
+Qed.
+
+
+
+
+
+
+
+
+
+
