progs/verif_sha_bdo2.v
@@ -1,0 +1,101 @@
+Require Import floyd.proofauto.
+Require Import progs.sha.
+Require Import progs.SHA256.
+Require Import progs.sha_lemmas.
+Require Import progs.spec_sha.
+Local Open Scope logic.
+
+Lemma elim_globals_only:
+  forall Delta g i t rho,
+  tc_environ Delta rho /\ (glob_types Delta) ! i = Some g ->
+  eval_var i t (globals_only rho) = eval_var i t rho.
+Admitted.
+
+Lemma sha256_block_data_order_return:
+forall (Espec : OracleKind) (hashed : list int) (delta : nat)
+  (data0 : list Z) (b : list int) (ctx data : val) (r_h : list int)
+  (r_Nl r_Nh : int) (r_data : list int) (r_num : int) (n : nat),
+length b = LBLOCK ->
+r_h = process_msg init_registers hashed ->
+length (intlist_to_Zlist hashed) =
+delta + Z.to_nat (Int.unsigned r_Nh * Int.modulus + Int.unsigned r_Nl) ->
+data0 = map Int.unsigned (firstn (Z.to_nat (Int.unsigned r_num)) r_data) ->
+length data0 < CBLOCK ->
+length hashed = (16 * n)%nat ->
+length r_data = CBLOCK ->
+length r_h = 8 ->
+isptr data ->
+semax (initialized _t Delta_loop1)
+  (PROP  ()
+   LOCAL ()
+   SEP 
+   (`(array_at tuint Tsh
+        (ZnthV tuint
+           (map2 Int.add (process_msg init_registers hashed)
+              (rnd_64 r_h K (rev (generate_word (rev b) 48))))) 0
+        (Zlength (process_msg init_registers hashed)) ctx);
+   `(array_at tuint Tsh (ZnthV tuint K) 0 (Zlength K))
+     (eval_var _K256 (tarray tuint 64));
+   `(array_at_ tuint Tsh 0 16) (eval_var _X (tarray tuint 16));
+   `(data_block (intlist_to_Zlist b) data);
+   `(field_mapsto Tsh t_struct_SHA256state_st _Nl ctx (Vint r_Nl));
+   `(field_mapsto Tsh t_struct_SHA256state_st _Nh ctx (Vint r_Nh));
+   `(array_at tuchar Tsh (ZnthV tuchar r_data) 0 (Zlength r_data)
+       (offset_val (Int.repr 40) ctx));
+   `(field_mapsto Tsh t_struct_SHA256state_st _num ctx (Vint r_num))))
+  (Sreturn None)
+  (frame_ret_assert
+     (function_body_ret_assert tvoid
+        (`(sha256state_ (process_block_abs b (S256abs hashed delta data0))
+             ctx) * `(data_block (intlist_to_Zlist b) data) *
+         `(array_at tuint Tsh (ZnthV tuint K) 0 (Zlength K))
+           (eval_var _K256 (tarray tuint 64))))
+     (stackframe_of f_sha256_block_data_order)).
+Proof.
+intros.
+forward. (* return; *)
+unfold frame_ret_assert; simpl.
+unfold sha256state_.
+set (regs := map2 Int.add (process_msg init_registers hashed)
+        (rnd_64 (process_msg init_registers hashed) K
+           (rev (generate_word (rev b) 48)))).
+repeat rewrite exp_sepcon1.
+apply exp_right with (regs, (r_Nl, (r_Nh, (r_data, r_num)))).
+simpl_typed_mapsto.
+unfold s256_relate, s256_h, s256_Nh, s256_Nl, s256_data, s256_num.
+unfold fst,snd.
+entailer!.
+* 
+apply process_msg_block; eauto.
+* 
+rewrite length_intlist_to_Zlist.
+rewrite app_length.
+rewrite H.
+rewrite length_intlist_to_Zlist in *.
+change CBLOCK with 64%nat.
+change LBLOCK with 16%nat.
+rewrite mult_plus_distr_l.
+change (4*16)%nat with 64%nat.
+omega.
+*
+exists (S n). rewrite app_length. rewrite H4, H.
+change LBLOCK with 16%nat.
+transitivity (16 * n + 16 * 1)%nat; [reflexivity | ].
+rewrite <- mult_plus_distr_l.
+rewrite plus_comm. reflexivity.
+*
+assert (Lregs: length regs = 8%nat)
+  by (subst; apply length_map2_add_rnd_64; auto).
+rewrite Zlength_correct; rewrite length_process_msg.
+rewrite (Zlength_correct regs); rewrite Lregs.
+simpl Z.of_nat.
+unfold stackframe_of; simpl.
+rewrite var_block_typed_mapsto_.
+normalize. simpl_typed_mapsto.
+change (Pos.to_nat 16) with 16%nat.
+unfold id.
+erewrite elim_globals_only
+  by (split; [eassumption | reflexivity]).
+apply andp_right; [ | cancel].
+apply prop_right; compute; congruence.
+Qed.
