progs/verif_sha_bdo3.v
@@ -1,0 +1,281 @@
+Require Import floyd.proofauto.
+Require Import progs.sha.
+Require Import progs.SHA256.
+Require Import progs.sha_lemmas.
+Require Import progs.spec_sha.
+Local Open Scope logic.
+
+Lemma and_mone':
+ forall x, Int.and x (Int.repr (-1)) = x.
+Proof.
+apply Int.and_mone.
+Qed.
+
+Lemma Sigma_1_eq: forall f_,
+  Sigma_1 f_ =
+            (Int.xor
+              (Int.xor
+                 (Int.or (Int.shl f_ (Int.repr 26))
+                    (Int.shru (Int.and f_ (Int.repr (-1)))
+                       (Int.sub (Int.repr 32) (Int.repr 26))))
+                 (Int.or (Int.shl f_ (Int.repr 21))
+                    (Int.shru (Int.and f_ (Int.repr (-1)))
+                       (Int.sub (Int.repr 32) (Int.repr 21)))))
+              (Int.or (Int.shl f_ (Int.repr 7))
+                 (Int.shru (Int.and f_ (Int.repr (-1)))
+                    (Int.sub (Int.repr 32) (Int.repr 7))))).
+Proof.
+intros.
+unfold Sigma_1, Sh.
+repeat rewrite and_mone'.
+repeat rewrite <- Int.or_ror by reflexivity.
+change (Int.sub (Int.repr 32) (Int.repr 26)) with (Int.repr 6).
+change (Int.sub (Int.repr 32) (Int.repr 21)) with (Int.repr 11).
+change (Int.sub (Int.repr 32) (Int.repr 7)) with (Int.repr 25).
+reflexivity.
+Qed.
+
+Lemma  Sigma_0_eq: forall b_,
+   Sigma_0 b_ = 
+      (Int.xor
+        (Int.xor
+           (Int.or (Int.shl b_ (Int.repr 30))
+              (Int.shru (Int.and b_ (Int.repr (-1)))
+                 (Int.sub (Int.repr 32) (Int.repr 30))))
+           (Int.or (Int.shl b_ (Int.repr 19))
+              (Int.shru (Int.and b_ (Int.repr (-1)))
+                 (Int.sub (Int.repr 32) (Int.repr 19)))))
+        (Int.or (Int.shl b_ (Int.repr 10))
+           (Int.shru (Int.and b_ (Int.repr (-1)))
+              (Int.sub (Int.repr 32) (Int.repr 10))))).
+Proof.
+intros.
+unfold Sigma_0, Sh.
+repeat rewrite and_mone'.
+repeat rewrite <- Int.or_ror by reflexivity.
+change (Int.sub (Int.repr 32) (Int.repr 19)) with (Int.repr 13).
+change (Int.sub (Int.repr 32) (Int.repr 10)) with (Int.repr 22).
+change (Int.sub (Int.repr 32) (Int.repr 30)) with (Int.repr 2).
+reflexivity.
+Qed.
+
+Lemma Ch_eq: forall f_ g_ h_,
+  Ch f_ g_ h_ =
+        (Int.xor (Int.and f_ g_) (Int.and (Int.not f_) h_)).
+Proof. reflexivity.
+Qed.
+
+Lemma Maj_eq:
+  forall b c d, 
+  Maj b c d =
+  (Int.xor (Int.xor (Int.and b c) (Int.and b d)) (Int.and c d)).
+Proof.
+intros.
+unfold Maj.
+rewrite (Int.xor_commut) at 1.
+rewrite Int.xor_assoc. auto.
+Qed.
+
+Lemma rearrange_aux:
+ forall h f c k l,
+ Int.add (Int.add (Int.add (Int.add h f) c) k) l =
+Int.add (Int.add (Int.add (Int.add l h) f) c) k.
+Proof.
+intros.
+rewrite <- (Int.add_commut l).
+repeat rewrite (Int.add_assoc h).
+rewrite <- (Int.add_assoc l).
+repeat rewrite (Int.add_assoc (Int.add l h)).
+reflexivity.
+Qed.
+
+Lemma rearrange_aux2: 
+forall (Espec : OracleKind) (i : nat)(w k : int)
+  (regs' : registers) (a b c d e f g h : int) (eqofs : val -> Prop),
+i < 16 ->
+semax (initialized _Ki (initialized _l (initialized _l' Delta_loop1)))
+  (PROP  ()
+   LOCAL  (`eqofs (eval_id _data); `(eq (Vint w)) (eval_id _l);
+   `(eq (Vint k)) (eval_id _Ki);
+   `(eq (Vint (Int.repr (Z.of_nat i)))) (eval_id _i);
+   `(eq (map Vint [a, b, c, d, e, f, g, h]))
+     (`cons (eval_id _a)
+        (`cons (eval_id _b)
+           (`cons (eval_id _c)
+              (`cons (eval_id _d)
+                 (`cons (eval_id _e)
+                    (`cons (eval_id _f)
+                       (`cons (eval_id _g) (`cons (eval_id _h) `[])))))))))
+   SEP()) rearrange_regs
+  (normal_ret_assert
+     (PROP  (S i <= 16)
+      LOCAL  (`(eq (Vint (Int.repr (Z.of_nat i)))) (eval_id _i);
+      `eqofs (eval_id _data);
+      `(eq (map Vint (rnd_function [a, b, c, d, e, f, g, h]  k w)))
+        (`cons (eval_id _a)
+           (`cons (eval_id _b)
+              (`cons (eval_id _c)
+                 (`cons (eval_id _d)
+                    (`cons (eval_id _e)
+                       (`cons (eval_id _f)
+                          (`cons (eval_id _g) (`cons (eval_id _h) `[])))))))))
+        SEP())).
+Proof.
+{
+intros.
+name a_ _a.
+name b_ _b.
+name c_ _c.
+name d_ _d.
+name e_ _e.
+name f_ _f.
+name g_ _g.
+name h_ _h.
+name l_ _l.
+name Ki _Ki.
+name i_ _i.
+name T1 _T1.
+name T2 _T2.
+name data_ _data.
+unfold Delta_loop1; simplify_Delta.
+simpl.
+unfold rearrange_regs.
+repeat forward.
+simpl eval_binop.
+go_lower0;
+repeat (apply derives_extract_prop; intro);
+repeat apply andp_right; try apply prop_right; auto.
+decompose [and] H2; clear H2; subst.
+inv H17.
+repeat match goal with 
+ | H: eval_id _ rho = _ |- _ => rewrite H in *; clear H
+ | H: _ = eval_id _ rho |- _ => rewrite <- H in *; clear H
+end.
+repeat split; auto.
+clear H13 H0 rho H1 H19 Delta.
+clear.
+cbv beta iota delta [sem_and sem_notint sem_or sem_shl sem_shr sem_or sem_add sem_xor]; simpl.
+repeat rewrite <- Sigma_1_eq.
+repeat rewrite <- Sigma_0_eq.
+repeat rewrite <- Ch_eq.
+repeat rewrite <- Maj_eq.
+repeat rewrite (rearrange_aux h).
+reflexivity.
+}
+Admitted.  (* can't Qed, because it goes over 2 gigabytes *)
+
+Lemma rearrange_regs_proof:
+ forall (Espec: OracleKind) i (data: val) bl regs
+ (Hdata: isptr data)
+ (H: length bl = LBLOCK)
+ (H0: i < 16), 
+ semax (initialized _Ki (initialized _l (initialized _l' Delta_loop1)))
+  (PROP  ()
+   LOCAL 
+   (`(eq (offset_val (Int.repr (Zsucc (Z.of_nat i) * 4)) data)) (eval_id _data);
+   `(eq (Vint (big_endian_integer
+             (fun z : Z =>
+              force_option Int.zero
+                (ZnthV tuchar (map Int.repr (intlist_to_Zlist (map swap bl)))
+                   (z + Z.of_nat i * 4))))))
+       (eval_id _l);
+   `(eq (nth_error K i)) (`Some  (`force_int (eval_id _Ki)));
+   `(eq (Vint (Int.repr (Z.of_nat i)))) (eval_id _i);
+   `(eq (map Vint (rnd_64 regs K (firstn i bl))))
+     (`cons (eval_id _a)
+        (`cons (eval_id _b)
+           (`cons (eval_id _c)
+              (`cons (eval_id _d)
+                 (`cons (eval_id _e)
+                    (`cons (eval_id _f)
+                       (`cons (eval_id _g) (`cons (eval_id _h) `[])))))))))
+   SEP()) rearrange_regs
+  (normal_ret_assert
+     (PROP  (S i <= 16)
+      LOCAL  (`(eq (Vint (Int.repr (Z.succ (Z.of_nat i) - 1)))) (eval_id _i);
+      `(eq (offset_val (Int.repr (Z.succ (Z.of_nat i) * 4)) data)) (eval_id _data);
+      `(eq (map Vint (rnd_64 regs K (firstn (S i) bl))))
+        (`cons (eval_id _a)
+           (`cons (eval_id _b)
+              (`cons (eval_id _c)
+                 (`cons (eval_id _d)
+                    (`cons (eval_id _e)
+                       (`cons (eval_id _f)
+                          (`cons (eval_id _g) (`cons (eval_id _h) `[])))))))))
+        SEP())).
+Proof.
+intros.
+name a_ _a.
+name b_ _b.
+name c_ _c.
+name d_ _d.
+name e_ _e.
+name f_ _f.
+name g_ _g.
+name h_ _h.
+name l_ _l.
+name Ki _Ki.
+name i_ _i.
+name T1 _T1.
+name T2 _T2.
+name data_ _data.
+assert (exists w, nth_error bl i = Some w).
+ apply assert_lemmas.nth_error_in_bounds.
+change LBLOCK with 16 in H; omega.
+destruct H1 as [w H1].
+assert (exists k, nth_error K i = Some k).
+ apply assert_lemmas.nth_error_in_bounds.
+compute; split; omega.
+destruct H2 as [k H2].
+set (Delta := initialized _Ki (initialized _l (initialized _l' Delta_loop1))).
+set (Delta' := initialized _Ki (initialized _l (initialized _l' Delta_loop1))).
+assert (Delta' = Delta) by reflexivity.
+revert H3.
+revert Delta.
+cbv delta [Delta_loop1].
+simplify_Delta.
+intro HDelta'.
+match goal with
+         | |- semax ?D _ _ _  =>
+               abbreviate D : tycontext as Delta
+end.
+assert (HDelta'': Delta' = Delta) by reflexivity.
+clear HDelta'.
+rewrite (rnd_64_S _ _ _ _ _ H2 H1).
+forget (rnd_64 regs K (firstn i bl)) as regs'.
+apply semax_pre with
+  (PROP  (exists a, exists b, exists c, exists d, 
+              exists e, exists f, exists g, exists h,
+                regs' = [a,b,c,d,e,f,g,h])
+   LOCAL 
+   (`(eq (offset_val (Int.repr (Z.succ (Z.of_nat i) * 4)) data))
+      (eval_id _data);
+   `(eq (Vint w)) (eval_id _l);
+   `(eq (Vint k)) (eval_id _Ki);
+   `(eq (Vint (Int.repr (Z.of_nat i)))) (eval_id _i);
+   `(eq (map Vint regs'))
+     (`cons (eval_id _a)
+        (`cons (eval_id _b)
+           (`cons (eval_id _c)
+              (`cons (eval_id _d)
+                 (`cons (eval_id _e)
+                    (`cons (eval_id _f)
+                       (`cons (eval_id _g) (`cons (eval_id _h) `[])))))))))
+   SEP()).
+abstract (entailer;
+  [(exists a_, b_, c_, d_, e_, f_, g_, h_;
+    clear - H4; rename H4 into H0;
+    do 8 (destruct regs' as [ | ? regs']; [inv H0 | ]);
+    destruct regs'; inv H0; reflexivity)
+  | apply nth_big_endian_integer''; auto 
+  | congruence]).
+apply semax_extract_PROP; 
+   intros [a [b [c [d [e [f [g [h Hregs]]]]]]]].
+forget (eq (offset_val (Int.repr (Z.succ (Z.of_nat i) * 4)) data)) as eqofs.
+clear Hdata data.
+replace (Z.succ (Z.of_nat i) - 1)%Z with (Z.of_nat i) by (clear; omega).
+rewrite <- HDelta''; unfold Delta'.
+clear Delta' HDelta'' Delta.
+subst regs'.
+eapply rearrange_aux2; eassumption. 
+Qed.
